src/main.fst
@@ -18,8 +18,11 @@ module U8 = FStar.UInt8
 inline_for_extraction noextract
 let (!$) = C.String.of_literal
 
-val max_u32 : U32.t
+val max_u32: U32.t
 let max_u32 = 4294967295ul
+
+val max_u8: U8.t
+let max_u8 = 255uy
 
 // https://docs.oasis-open.org/mqtt/mqtt/v5.0/os/mqtt-v5.0-os.html#_Toc3901022
 // 2.1.2 MQTT Control Packet type
@@ -105,7 +108,7 @@ let is_valid_message_type_check message_type =
     0uy
 
 type type_mqtt_control_packets_restrict =
-  v:type_mqtt_control_packets{U8.eq (is_valid_message_type_check v) 0uy || U8.eq v 255uy}
+  v:type_mqtt_control_packets{U8.eq (is_valid_message_type_check v) 0uy || U8.eq v max_u8}
 
 
 // https://docs.oasis-open.org/mqtt/mqtt/v5.0/os/mqtt-v5.0-os.html#_Toc3901022
@@ -145,7 +148,7 @@ let is_valid_dup_flag dup_flag =
     0uy
 
 type type_dup_flags_restrict =
-  dup_flag: type_dup_flags{U8.eq (is_valid_dup_flag dup_flag) 0uy || U8.eq dup_flag 255uy}
+  dup_flag: type_dup_flags{U8.eq (is_valid_dup_flag dup_flag) 0uy || U8.eq dup_flag max_u8}
 
 // https://docs.oasis-open.org/mqtt/mqtt/v5.0/os/mqtt-v5.0-os.html
 // 3.3.1.2 QoS
@@ -167,7 +170,7 @@ let is_valid_qos_flag qos_flag =
     0uy
 
 type type_qos_flags_restrict =
-  qos_flag: type_qos_flags{U8.eq (is_valid_qos_flag qos_flag) 0uy || U8.eq qos_flag 255uy}
+  qos_flag: type_qos_flags{U8.eq (is_valid_qos_flag qos_flag) 0uy || U8.eq qos_flag max_u8}
 
 // https://docs.oasis-open.org/mqtt/mqtt/v5.0/os/mqtt-v5.0-os.html
 // 3.3.1.3 RETAIN
@@ -185,124 +188,14 @@ let is_valid_retain_flag retain_flag =
     0uy
 
 type type_retain_flags_restrict =
-  retain_flag: type_retain_flags{U8.eq (is_valid_retain_flag retain_flag) 0uy || U8.eq retain_flag 255uy}
-
-val is_valid_connect_flag: flag:U8.t -> (r:U8.t{U8.v r <= 1})
-let is_valid_connect_flag flag =
- if (flag <> define_flag_CONNECT) then
- 1uy
- else
- 0uy
-
-val is_valid_connack_flag: flag:U8.t -> (r:U8.t{U8.v r <= 1})
-let is_valid_connack_flag flag =
- if (flag <> define_flag_CONNACK) then
- 1uy
- else
- 0uy
-
-val is_valid_puback_flag: flag:U8.t -> (r:U8.t{U8.v r <= 1})
-let is_valid_puback_flag flag =
- if (flag <> define_flag_PUBACK) then
- 1uy
- else
- 0uy
-
-val is_valid_pubrec_flag: flag:U8.t -> (r:U8.t{U8.v r <= 1})
-let is_valid_pubrec_flag flag =
- if (flag <> define_flag_PUBREC) then
- 1uy
- else
- 0uy
-
-val is_valid_pubrel_flag: flag:U8.t -> (r:U8.t{U8.v r <= 1})
-let is_valid_pubrel_flag flag =
- if (flag <> define_flag_PUBREL) then
- 1uy
- else
- 0uy
-
-val is_valid_pubcomp_flag: flag:U8.t -> (r:U8.t{U8.v r <= 1})
-let is_valid_pubcomp_flag flag =
- if (flag <> define_flag_PUBCOMP) then
- 1uy
- else
- 0uy
-
-val is_valid_subscribe_flag: flag:U8.t -> (r:U8.t{U8.v r <= 1})
-let is_valid_subscribe_flag flag =
- if (flag <> define_flag_SUBSCRIBE) then
- 1uy
- else
- 0uy
-
-val is_valid_suback_flag: flag:U8.t -> (r:U8.t{U8.v r <= 1})
-let is_valid_suback_flag flag =
- if (flag <> define_flag_SUBACK) then
- 1uy
- else
- 0uy
-
-val is_valid_unsubscribe_flag: flag:U8.t -> (r:U8.t{U8.v r <= 1})
-let is_valid_unsubscribe_flag flag =
- if (flag <> define_flag_UNSUBSCRIBE) then
- 1uy
- else
- 0uy
-
-val is_valid_unsuback_flag: flag:U8.t -> (r:U8.t{U8.v r <= 1})
-let is_valid_unsuback_flag flag =
- if (flag <> define_flag_UNSUBACK) then
- 1uy
- else
- 0uy
-
-val is_valid_pingreq_flag: flag:U8.t -> (r:U8.t{U8.v r <= 1})
-let is_valid_pingreq_flag flag =
- if (flag <> define_flag_PINGREQ) then
- 1uy
- else
- 0uy
-
-val is_valid_pingresp_flag: flag:U8.t -> (r:U8.t{U8.v r <= 1})
-let is_valid_pingresp_flag flag =
- if (flag <> define_flag_PINGRESP) then
- 1uy
- else
- 0uy
-
-val is_valid_disconnect_flag: flag:U8.t -> (r:U8.t{U8.v r <= 1})
-let is_valid_disconnect_flag flag =
- if (flag <> define_flag_DISCONNECT) then
- 1uy
- else
- 0uy
-
-val is_valid_auth_flag: flag:U8.t -> (r:U8.t{U8.v r <= 1})
-let is_valid_auth_flag flag =
- if (flag <> define_flag_AUTH) then
- 1uy
- else
- 0uy
+  retain_flag: type_retain_flags{U8.eq (is_valid_retain_flag retain_flag) 0uy || U8.eq retain_flag max_u8}
 
 type type_flag_restrict =
- flag: U8.t{
- U8.eq (is_valid_connect_flag flag) 0uy ||
- U8.eq (is_valid_connack_flag flag) 0uy ||
- U8.eq (is_valid_puback_flag flag) 0uy ||
- U8.eq (is_valid_pubrec_flag flag) 0uy ||
- U8.eq (is_valid_pubrel_flag flag) 0uy ||
- U8.eq (is_valid_pubcomp_flag flag) 0uy ||
- U8.eq (is_valid_subscribe_flag flag) 0uy ||
- U8.eq (is_valid_suback_flag flag) 0uy ||
- U8.eq (is_valid_unsubscribe_flag flag) 0uy ||
- U8.eq (is_valid_unsuback_flag flag) 0uy ||
- U8.eq (is_valid_pingreq_flag flag) 0uy ||
- U8.eq (is_valid_pingresp_flag flag) 0uy ||
- U8.eq (is_valid_disconnect_flag flag) 0uy ||
- U8.eq (is_valid_auth_flag flag) 0uy ||
- U8.eq flag 255uy
- }
+  flag: U8.t{
+    U8.eq flag 0b0000uy ||
+    U8.eq flag 0b0010uy ||
+    U8.eq flag max_u8
+}
 
 type type_remaining_length =
   (remaining_length: U32.t{U32.v remaining_length <= 268435455 || U32.eq remaining_length max_u32})
@@ -314,7 +207,6 @@ assume val print_hex (i:U8.t): Stack unit
   (requires (fun h -> true))
   (ensures (fun h0 ret h1 -> true))
 
-// TODO: テストする
 val slice_byte:
   byte:U8.t
   -> a:U8.t{U8.v a <= 7}
@@ -381,7 +273,6 @@ let is_valid_decoding_packet_check ptr_for_decoding_packets bytes_length =
     (requires (fun h -> inv h (U32.v i)))
     (ensures (fun _ _ _ -> true))
   =
-    // TODO: 入れ子がわかりにくい
     let ptr_status_v = ptr_status.(0ul) in
     let bytes_length_u32 = uint8_to_uint32(bytes_length) in
       if (U8.eq ptr_status_v 0uy) then
@@ -411,7 +302,7 @@ let is_valid_decoding_packet_check ptr_for_decoding_packets bytes_length =
                                   )
                               ) else
                                   (
-                                    if (U8.lt decoding_packet 128uy || U8.gt decoding_packet 255uy) then
+                                    if (U8.lt decoding_packet 128uy || U8.gt decoding_packet max_u8) then
                                       (
                                         // print_string "err3\n";
                                         ptr_status.(0ul) <- 3uy
@@ -531,9 +422,8 @@ let decodeing_variable_bytes ptr_for_decoding_packets bytes_length =
 // x (1byte) + (msg len byte 3 or 4) + (100012byte) = 100016
 // (1byte) + (3byte) + (100012byte) = 100016
 
-// // TODO: 値域の設定
 val get_remaining_length: bytes_length:U8.t{U8.v bytes_length >= 1 && U8.v bytes_length <= 4} -> ptr_for_decoding_packets: B.buffer U8.t -> packet_size:U32.t{1 <= U32.v packet_size}
-  -> Stack (remaining_length:type_remaining_length) // TODO: エラーの返り値をどうするか
+  -> Stack (remaining_length:type_remaining_length)
   (requires fun h0 -> B.live h0 ptr_for_decoding_packets /\ B.length ptr_for_decoding_packets = 4)
   (ensures fun _ _ _ -> true)
 let get_remaining_length bytes_length ptr_for_decoding_packets packet_size =
@@ -637,96 +527,28 @@ let get_message_type message_type_bits =
   if (U8.eq (is_valid_message_type_check message_type_bits) 0uy) then
     message_type_bits
   else
-    255uy
+    max_u8
 
 val get_dup_flag: dup_flag_bits: U8.t -> type_dup_flags
 let get_dup_flag dup_flag_bits =
   if (U8.eq (is_valid_dup_flag dup_flag_bits) 0uy) then
     dup_flag_bits
   else
-    255uy
+    max_u8
 
 val get_qos_flag: qos_flag_bits: U8.t -> type_qos_flags
 let get_qos_flag qos_flag_bits =
   if (U8.eq (is_valid_qos_flag qos_flag_bits) 0uy) then
     qos_flag_bits
   else
-    255uy
+    max_u8
 
 val get_retain_flag: retain_flag_bits: U8.t -> type_retain_flags
 let get_retain_flag retain_flag_bits =
   if (U8.eq (is_valid_retain_flag retain_flag_bits) 0uy) then
     retain_flag_bits
   else
-    255uy
-
-val get_flag : flags_bits:U8.t -> type_flag_restrict
-let get_flag flags_bits =
-  if (U8.eq (is_valid_connect_flag flags_bits) 0uy) then
-    flags_bits
-  else if (U8.eq (is_valid_connack_flag flags_bits) 0uy) then
-    flags_bits
-  else if (U8.eq (is_valid_puback_flag flags_bits) 0uy) then
-    flags_bits
-  else if (U8.eq (is_valid_pubrec_flag flags_bits) 0uy) then
-   flags_bits
-  else if (U8.eq (is_valid_pubrel_flag flags_bits) 0uy) then
-   flags_bits
-  else if (U8.eq (is_valid_pubcomp_flag flags_bits) 0uy) then
-   flags_bits
-  else if (U8.eq (is_valid_subscribe_flag flags_bits) 0uy) then
-   flags_bits
-  else if (U8.eq (is_valid_suback_flag flags_bits) 0uy) then
-   flags_bits
-  else if (U8.eq (is_valid_unsubscribe_flag flags_bits) 0uy) then
-   flags_bits
-  else if (U8.eq (is_valid_unsuback_flag flags_bits) 0uy) then
-   flags_bits
-  else if (U8.eq (is_valid_pingreq_flag flags_bits) 0uy) then
-   flags_bits
-  else if (U8.eq (is_valid_pingresp_flag flags_bits) 0uy) then
-   flags_bits
-  else if (U8.eq (is_valid_disconnect_flag flags_bits) 0uy) then
-   flags_bits
-  else if (U8.eq (is_valid_auth_flag flags_bits) 0uy) then
-   flags_bits
-  else
-   255uy
-
-val get_message_name: message_type:type_mqtt_control_packets_restrict -> r:type_message_name_restrict
-let get_message_name message_type =
-  if (U8.eq message_type define_mqtt_control_packet_CONNECT) then
-    define_mqtt_control_packet_CONNECT_label
-  else if (U8.eq message_type define_mqtt_control_packet_CONNACK) then
-    define_mqtt_control_packet_CONNACK_label
-  else if (U8.eq message_type define_mqtt_control_packet_PUBLISH) then
-    define_mqtt_control_packet_PUBLISH_label
-  else if (U8.eq message_type define_mqtt_control_packet_PUBACK) then
-    define_mqtt_control_packet_PUBACK_label
-  else if (U8.eq message_type define_mqtt_control_packet_PUBREC) then
-    define_mqtt_control_packet_PUBREC_label
-  else if (U8.eq message_type define_mqtt_control_packet_PUBREL) then
-    define_mqtt_control_packet_PUBREL_label
-  else if (U8.eq message_type define_mqtt_control_packet_PUBCOMP) then
-    define_mqtt_control_packet_PUBCOMP_label
-  else if (U8.eq message_type define_mqtt_control_packet_SUBSCRIBE) then
-    define_mqtt_control_packet_SUBSCRIBE_label
-  else if (U8.eq message_type define_mqtt_control_packet_SUBACK) then
-    define_mqtt_control_packet_SUBACK_label
-  else if (U8.eq message_type define_mqtt_control_packet_UNSUBSCRIBE) then
-    define_mqtt_control_packet_UNSUBSCRIBE_label
-  else if (U8.eq message_type define_mqtt_control_packet_UNSUBACK) then
-    define_mqtt_control_packet_UNSUBACK_label
-  else if (U8.eq message_type define_mqtt_control_packet_PINGREQ) then
-    define_mqtt_control_packet_PINGREQ_label
-  else if (U8.eq message_type define_mqtt_control_packet_PINGRESP) then
-    define_mqtt_control_packet_PINGRESP_label
-  else if (U8.eq message_type define_mqtt_control_packet_DISCONNECT) then
-    define_mqtt_control_packet_DISCONNECT_label
-  else if (U8.eq message_type define_mqtt_control_packet_AUTH) then
-    define_mqtt_control_packet_AUTH_label
-  else
-    !$""
+    max_u8
 
 type struct_flags = {
   flag: type_flag_restrict;
@@ -735,12 +557,205 @@ type struct_flags = {
   retain_flag: type_retain_flags_restrict;
 }
 
+type struct_fixed_header_constant = {
+  message_type_constant: type_mqtt_control_packets_restrict;
+  message_name_constant: type_message_name_restrict;
+  flags_constant: struct_flags;
+}
+
 type struct_fixed_header = {
-  message_name: type_message_name_restrict;
   message_type: type_mqtt_control_packets_restrict;
+  message_name: type_message_name_restrict;
   flags: struct_flags;
   remaining_length: type_remaining_length;
   error_message: type_error_message_restrict;
+}
+
+val is_valid_flag: s:struct_fixed_header_constant -> flag: type_flag_restrict -> bool
+let is_valid_flag s flag = U8.eq s.flags_constant.flag flag
+
+val struct_fixed_connect: u:unit -> struct_fixed_header_constant
+let struct_fixed_connect u = {
+  message_type_constant = define_mqtt_control_packet_CONNECT;
+  message_name_constant = define_mqtt_control_packet_CONNECT_label;
+  flags_constant = {
+    flag = define_flag_CONNECT;
+    dup_flag = max_u8;
+    qos_flag = max_u8;
+    retain_flag = max_u8;
+  };
+}
+
+val struct_fixed_connack: u:unit -> struct_fixed_header_constant
+let struct_fixed_connack u = {
+  message_type_constant = define_mqtt_control_packet_CONNACK;
+  message_name_constant = define_mqtt_control_packet_CONNACK_label;
+  flags_constant = {
+    flag = define_flag_CONNACK;
+    dup_flag = max_u8;
+    qos_flag = max_u8;
+    retain_flag = max_u8;
+  };
+}
+
+val struct_fixed_publish:
+  (dup_flag:type_dup_flags_restrict)
+  -> (qos_flag:type_qos_flags_restrict)
+  -> (retain_flag:type_retain_flags_restrict)
+  -> struct_fixed_header_constant
+let struct_fixed_publish dup_flag qos_flag retain_flag = {
+  message_type_constant = define_mqtt_control_packet_PUBLISH;
+  message_name_constant = define_mqtt_control_packet_PUBLISH_label;
+  flags_constant = {
+    flag = max_u8;
+    dup_flag = dup_flag;
+    qos_flag = qos_flag;
+    retain_flag = retain_flag;
+  };
+}
+
+val struct_fixed_puback: u:unit -> struct_fixed_header_constant
+let struct_fixed_puback u = {
+  message_type_constant = define_mqtt_control_packet_PUBACK;
+  message_name_constant = define_mqtt_control_packet_PUBACK_label;
+  flags_constant = {
+    flag = define_flag_PUBACK;
+    dup_flag = max_u8;
+    qos_flag = max_u8;
+    retain_flag = max_u8;
+  };
+}
+
+val struct_fixed_pubrec: u:unit -> struct_fixed_header_constant
+let struct_fixed_pubrec u = {
+  message_type_constant = define_mqtt_control_packet_PUBREC;
+  message_name_constant = define_mqtt_control_packet_PUBREC_label;
+  flags_constant = {
+    flag = define_flag_PUBREC;
+    dup_flag = max_u8;
+    qos_flag = max_u8;
+    retain_flag = max_u8;
+  };
+}
+
+val struct_fixed_pubrel: u:unit -> struct_fixed_header_constant
+let struct_fixed_pubrel u = {
+  message_type_constant = define_mqtt_control_packet_PUBREL;
+  message_name_constant = define_mqtt_control_packet_PUBREL_label;
+  flags_constant = {
+    flag = define_flag_PUBREL;
+    dup_flag = max_u8;
+    qos_flag = max_u8;
+    retain_flag = max_u8;
+  };
+}
+
+val struct_fixed_pubcomp: u:unit -> struct_fixed_header_constant
+let struct_fixed_pubcomp u = {
+  message_type_constant = define_mqtt_control_packet_PUBCOMP;
+  message_name_constant = define_mqtt_control_packet_PUBCOMP_label;
+  flags_constant = {
+    flag = define_flag_PUBCOMP;
+    dup_flag = max_u8;
+    qos_flag = max_u8;
+    retain_flag = max_u8;
+  };
+}
+
+val struct_fixed_subscribe: u:unit -> struct_fixed_header_constant
+let struct_fixed_subscribe u = {
+  message_type_constant = define_mqtt_control_packet_SUBSCRIBE;
+  message_name_constant = define_mqtt_control_packet_SUBSCRIBE_label;
+  flags_constant = {
+    flag = define_flag_SUBSCRIBE;
+    dup_flag = max_u8;
+    qos_flag = max_u8;
+    retain_flag = max_u8;
+  };
+}
+
+val struct_fixed_suback: u:unit -> struct_fixed_header_constant
+let struct_fixed_suback u = {
+  message_type_constant = define_mqtt_control_packet_SUBACK;
+  message_name_constant = define_mqtt_control_packet_SUBACK_label;
+  flags_constant = {
+    flag = define_flag_SUBACK;
+    dup_flag = max_u8;
+    qos_flag = max_u8;
+    retain_flag = max_u8;
+  };
+}
+
+val struct_fixed_unsubscribe: u:unit -> struct_fixed_header_constant
+let struct_fixed_unsubscribe u = {
+  message_type_constant = define_mqtt_control_packet_UNSUBSCRIBE;
+  message_name_constant = define_mqtt_control_packet_UNSUBSCRIBE_label;
+  flags_constant = {
+    flag = define_flag_UNSUBSCRIBE;
+    dup_flag = max_u8;
+    qos_flag = max_u8;
+    retain_flag = max_u8;
+  };
+}
+
+val struct_fixed_unsuback: u:unit -> struct_fixed_header_constant
+let struct_fixed_unsuback u = {
+  message_type_constant = define_mqtt_control_packet_UNSUBACK;
+  message_name_constant = define_mqtt_control_packet_UNSUBACK_label;
+  flags_constant = {
+    flag = define_flag_UNSUBACK;
+    dup_flag = max_u8;
+    qos_flag = max_u8;
+    retain_flag = max_u8;
+  };
+}
+
+val struct_fixed_pingreq: u:unit -> struct_fixed_header_constant
+let struct_fixed_pingreq u = {
+  message_type_constant = define_mqtt_control_packet_PINGREQ;
+  message_name_constant = define_mqtt_control_packet_PINGREQ_label;
+  flags_constant = {
+    flag = define_flag_PINGREQ;
+    dup_flag = max_u8;
+    qos_flag = max_u8;
+    retain_flag = max_u8;
+  };
+}
+
+val struct_fixed_pingresp: u:unit -> struct_fixed_header_constant
+let struct_fixed_pingresp u = {
+  message_type_constant = define_mqtt_control_packet_PINGRESP;
+  message_name_constant = define_mqtt_control_packet_PINGRESP_label;
+  flags_constant = {
+    flag = define_flag_PINGRESP;
+    dup_flag = max_u8;
+    qos_flag = max_u8;
+    retain_flag = max_u8;
+  };
+}
+
+val struct_fixed_disconnect: u:unit -> struct_fixed_header_constant
+let struct_fixed_disconnect u = {
+  message_type_constant = define_mqtt_control_packet_DISCONNECT;
+  message_name_constant = define_mqtt_control_packet_DISCONNECT_label;
+  flags_constant = {
+    flag = define_flag_DISCONNECT;
+    dup_flag = max_u8;
+    qos_flag = max_u8;
+    retain_flag = max_u8;
+  };
+}
+
+val struct_fixed_auth: u:unit -> struct_fixed_header_constant
+let struct_fixed_auth u = {
+  message_type_constant = define_mqtt_control_packet_AUTH;
+  message_name_constant = define_mqtt_control_packet_AUTH_label;
+  flags_constant = {
+    flag = define_flag_AUTH;
+    dup_flag = max_u8;
+    qos_flag = max_u8;
+    retain_flag = max_u8;
+  };
 }
 
 val bytes_loop: request: B.buffer U8.t -> packet_size: U32.t -> Stack struct_fixed_header
@@ -825,94 +840,168 @@ let bytes_loop request packet_size =
   let fixed_header_first_one_byte = ptr_fixed_header_first_one_byte.(0ul) in
   let message_type_bits: U8.t = slice_byte fixed_header_first_one_byte 0uy 4uy in
   let message_type: type_mqtt_control_packets_restrict = get_message_type message_type_bits in
-  let flags_bits: U8.t = slice_byte fixed_header_first_one_byte 4uy 8uy in
-  let flag: type_flag_restrict = get_flag flags_bits in
-  let dup_flag: type_dup_flags_restrict =
-   (
-    if (U8.eq message_type define_mqtt_control_packet_PUBLISH) then
-        let dup_flag_bits: U8.t = slice_byte fixed_header_first_one_byte 4uy 5uy in
-        get_dup_flag dup_flag_bits
-    else
-      255uy
-    ) in
-  let qos_flag: type_qos_flags_restrict =
-   (
-    if (U8.eq message_type define_mqtt_control_packet_PUBLISH) then
-        let qos_flag_bits: U8.t = slice_byte fixed_header_first_one_byte 5uy 7uy in
-        get_qos_flag qos_flag_bits
-    else
-      255uy
-    ) in
-  let retain_flag: type_retain_flags_restrict =
-   (
-    if (U8.eq message_type define_mqtt_control_packet_PUBLISH) then
-      let retain_flag_bits: U8.t = slice_byte fixed_header_first_one_byte 7uy 8uy in
-        get_retain_flag retain_flag_bits
-    else
-      255uy
-    ) in
   let remaining_length: type_remaining_length
     = ptr_remaining_length.(0ul) in
-  let message_name: type_message_name_restrict = get_message_name message_type in
-  let is_valid_message_type: U8.t = is_valid_message_type_check message_type in
-  let have_error: bool =
-    (U8.eq status 1uy) ||
-    (U8.eq message_type 255uy) ||
-    // (U32.eq (C.String.strlen message_name) 0ul) ||
-    (U8.eq flag 255uy) ||
-    (U8.eq message_type define_mqtt_control_packet_PUBLISH && U8.eq dup_flag 255uy) ||
-    (U8.eq message_type define_mqtt_control_packet_PUBLISH && U8.eq qos_flag 255uy) ||
-    (U8.eq message_type define_mqtt_control_packet_PUBLISH && U8.eq retain_flag 255uy) in
-  if (have_error = true) then
+  if (U8.eq message_type define_mqtt_control_packet_PUBLISH) then
     (
-      let data: struct_fixed_header = {
-            message_name = !$"";
-            message_type = 255uy;
+      let dup_flag: type_dup_flags_restrict =
+      (
+        if (U8.eq message_type define_mqtt_control_packet_PUBLISH) then
+            let dup_flag_bits: U8.t = slice_byte fixed_header_first_one_byte 4uy 5uy in
+            get_dup_flag dup_flag_bits
+        else
+          max_u8
+        ) in
+      let qos_flag: type_qos_flags_restrict =
+      (
+        if (U8.eq message_type define_mqtt_control_packet_PUBLISH) then
+            let qos_flag_bits: U8.t = slice_byte fixed_header_first_one_byte 5uy 7uy in
+            get_qos_flag qos_flag_bits
+        else
+          max_u8
+        ) in
+      let retain_flag: type_retain_flags_restrict =
+      (
+        if (U8.eq message_type define_mqtt_control_packet_PUBLISH) then
+          let retain_flag_bits: U8.t = slice_byte fixed_header_first_one_byte 7uy 8uy in
+            get_retain_flag retain_flag_bits
+        else
+          max_u8
+      ) in
+      let have_error: bool =
+          (U8.eq status 1uy) ||
+          (U8.eq message_type max_u8) ||
+          (U8.eq dup_flag max_u8) ||
+          (U8.eq qos_flag max_u8) ||
+          (U8.eq retain_flag max_u8) in
+      let error_message: type_error_message_restrict =
+        (
+          if (have_error) then (
+            if (U8.eq status 1uy) then
+              !$"remaining_length is invalid."
+            else if (U8.eq message_type max_u8) then
+              !$"message_type is invalid."
+            else if (U8.eq dup_flag max_u8) then
+              !$"dup_flag is invalid."
+            else if (U8.eq qos_flag max_u8) then
+              !$"qos_flag is invalid."
+            else if (U8.eq retain_flag max_u8) then
+              !$"retain_flag is invalid."
+            else
+              !$"unexpected error."
+          ) else
+            !$""
+        ) in
+      pop_frame ();
+      if (have_error) then
+        {
+          message_type = max_u8;
+          message_name = !$"";
+          flags = {
+            flag = max_u8;
+            dup_flag = max_u8;
+            qos_flag = max_u8;
+            retain_flag = max_u8;
+          };
+          remaining_length = 0ul;
+          error_message = error_message;
+        }
+      else
+        let data: struct_fixed_header_constant =
+          struct_fixed_publish dup_flag qos_flag retain_flag in
+          {
+            message_type = data.message_type_constant;
+            message_name = data.message_name_constant;
             flags = {
-              flag = 255uy;
-              dup_flag = 255uy;
-              qos_flag = 255uy;
-              retain_flag = 255uy;
+              flag = data.flags_constant.flag;
+              dup_flag = data.flags_constant.dup_flag;
+              qos_flag = data.flags_constant.qos_flag;
+              retain_flag = data.flags_constant.retain_flag;
             };
-            remaining_length = 0ul;
-            error_message =
-              if (U8.eq status 1uy) then
-                !$"remaining_length is invalid."
-              else if (U8.eq message_type 255uy) then
-                !$"message_type is invalid."
-              // else if (U32.eq (C.String.strlen message_name) 0ul) then
-              //   !$"message_name is invalid." ここは､message_typeを判定すれば不必要
-              else if (U8.eq flag 255uy) then
-                !$"flag is invalid."
-              else if (U8.eq message_type define_mqtt_control_packet_PUBLISH && U8.eq dup_flag 255uy) then
-                !$"dup_flag is invalid."
-              else if (U8.eq message_type define_mqtt_control_packet_PUBLISH && U8.eq qos_flag 255uy) then
-                !$"qos_flag is invalid."
-              else if (U8.eq message_type define_mqtt_control_packet_PUBLISH && U8.eq retain_flag 255uy) then
-                !$"retain_flag is invalid."
-              else
-                !$"unexpected error."
-          } in
-          pop_frame ();
-          data
+            remaining_length = remaining_length;
+            error_message = !$"";
+          }
     )
   else
     (
-      let flags: struct_flags = {
-          flag = flag;
-          dup_flag = dup_flag;
-          qos_flag = qos_flag;
-          retain_flag = retain_flag;
-      } in
-      let data: struct_fixed_header = {
-        message_name = message_name;
-        message_type = message_type;
-        flags = flags;
-        remaining_length = remaining_length;
-        error_message = !$"";
-      } in
-      pop_frame ();
-      (* return *) data
+      let flag: type_flag_restrict =
+        let v = slice_byte fixed_header_first_one_byte 4uy 8uy in
+          (
+            if (v <> 0b0000uy && v <> 0b0010uy && v <> max_u8) then
+              max_u8
+            else
+              v
+          ) in
+      let data: struct_fixed_header_constant =
+        if (U8.eq message_type define_mqtt_control_packet_CONNECT) then
+          struct_fixed_connect ()
+        else if (U8.eq message_type define_mqtt_control_packet_CONNACK) then
+          struct_fixed_connack ()
+        else if (U8.eq message_type define_mqtt_control_packet_PUBACK) then
+          struct_fixed_puback ()
+        else if (U8.eq message_type define_mqtt_control_packet_PUBREC) then
+          struct_fixed_pubrec ()
+        else if (U8.eq message_type define_mqtt_control_packet_PUBREL) then
+          struct_fixed_pubrel ()
+        else if (U8.eq message_type define_mqtt_control_packet_PUBCOMP) then
+          struct_fixed_pubcomp ()
+        else if (U8.eq message_type define_mqtt_control_packet_SUBSCRIBE) then
+          struct_fixed_subscribe ()
+        else if (U8.eq message_type define_mqtt_control_packet_SUBACK) then
+          struct_fixed_suback ()
+        else if (U8.eq message_type define_mqtt_control_packet_UNSUBSCRIBE) then
+          struct_fixed_unsubscribe ()
+        else if (U8.eq message_type define_mqtt_control_packet_UNSUBACK) then
+          struct_fixed_unsuback ()
+        else if (U8.eq message_type define_mqtt_control_packet_PINGREQ) then
+          struct_fixed_pingreq ()
+        else if (U8.eq message_type define_mqtt_control_packet_PINGRESP) then
+          struct_fixed_pingresp ()
+        else if (U8.eq message_type define_mqtt_control_packet_DISCONNECT) then
+          struct_fixed_disconnect ()
+        else
+          struct_fixed_auth () in
+      let have_error: bool =
+        (U8.eq status 1uy) ||
+        (U8.eq message_type max_u8) ||
+        (is_valid_flag data flag = false) in
+        pop_frame ();
+        if (have_error) then
+          (
+            {
+              message_type = max_u8;
+              message_name = !$"";
+              flags = {
+                flag = max_u8;
+                dup_flag = max_u8;
+                qos_flag = max_u8;
+                retain_flag = max_u8;
+              };
+              remaining_length = 0ul;
+              error_message =
+                if (U8.eq status 1uy) then
+                  !$"remaining_length is invalid."
+                else if (U8.eq message_type max_u8) then
+                  !$"message_type is invalid."
+                else if (is_valid_flag data flag = false) then
+                  !$"flag is invalid."
+                else
+                  !$"unexpected error."
+              }
+            )
+        else
+          {
+            message_type = data.message_type_constant;
+            message_name = data.message_name_constant;
+            flags = {
+              flag = data.flags_constant.flag;
+              dup_flag = data.flags_constant.dup_flag;
+              qos_flag = data.flags_constant.qos_flag;
+              retain_flag = data.flags_constant.retain_flag;
+            };
+            remaining_length = remaining_length;
+            error_message = !$"";
+          }
     )
 
 val parse (request: B.buffer U8.t) (packet_size: U32.t):
